CollapsingTowers/TwoLevelPCP/Effect.lean
@@ -1,0 +1,19 @@
+
+inductive Effects : Type where
+  | pure
+  | reflect
+
+@[simp]
+def union : Effects → Effects → Effects
+  | .pure, .pure => .pure
+  | .pure, .reflect => .reflect
+  | .reflect, .pure => .reflect
+  | .reflect, .reflect => .reflect
+
+instance : EmptyCollection Effects where emptyCollection := .pure
+
+instance : Union Effects where union := union
+
+theorem union_empty : forall φ : Effects, φ ∪ ∅ = φ := by
+  intro φ
+  cases φ <;> rfl
